IntegerStamp: add up & down masks, use 64 bits
Switch the lower and upper bounds of integer stamps
to use a 64 bit word rather than an unbounded intger.
Include the up and down masks (64 bit words) in the stamp.

Changed the definition of min and max integers
to be more ammenable to the word theories.
Proved backwards compatibility.

Graph/Stamp.thy
@@ -16,7 +16,7 @@ additionally provide a number of lemmas which help to prove future optimizations
 
 datatype Stamp = 
   VoidStamp
-  | IntegerStamp (stp_bits: nat) (stpi_lower: int) (stpi_upper: int)
+  | IntegerStamp (stp_bits: nat) (stpi_lower: int64) (stpi_upper: int64) (stpi_down: int64) (stpi_up: int64)
   (* | FloatStamp (stp_bits: nat) (stpf_lower: float) (stpf_upper: float) *)
   | KlassPointerStamp (stp_nonNull: bool) (stp_alwaysNull: bool)
   | MethodCountersPointerStamp (stp_nonNull: bool) (stp_alwaysNull: bool)
@@ -27,12 +27,12 @@ datatype Stamp =
 
 
 text \<open>To help with supporting masks in future, this constructor allows masks but ignores them.\<close>
-abbreviation IntegerStampM :: "nat \<Rightarrow> int \<Rightarrow> int \<Rightarrow> int64 \<Rightarrow> int64 \<Rightarrow> Stamp" where
-  "IntegerStampM b lo hi down up \<equiv> IntegerStamp b lo hi"
+abbreviation IntegerStampM :: "nat \<Rightarrow> int64 \<Rightarrow> int64 \<Rightarrow> int64 \<Rightarrow> int64 \<Rightarrow> Stamp" where
+  "IntegerStampM b lo hi down up \<equiv> IntegerStamp b lo hi down up"
 
 
 fun is_stamp_empty :: "Stamp \<Rightarrow> bool" where
-  "is_stamp_empty (IntegerStamp b lower upper) = (upper < lower)" |
+  "is_stamp_empty (IntegerStamp b lower upper down up) = (upper < lower)" |
   (* "is_stamp_empty (FloatStamp b lower upper) = (upper < lower)" | *)
   "is_stamp_empty x = False"
 
@@ -52,11 +52,53 @@ text \<open>Just like the IntegerStamp class, we need to know that our lo/hi bou
 (* TODO: should we have tight bounds for empty stamp, or just hi<lo?
    We could have: (lo = snd (bit_bounds bits) \<and> hi = fst (bit_bounds bits) 
  *)
+definition min_int :: "nat \<Rightarrow> int64" where
+  "min_int bits = set_bit (bits-1) 0"
+
+lemma min_int_push_bit:
+  assumes "0 < b \<and> b \<le> 64"
+  shows "-(2 ^ (b - 1)) = ((push_bit (b-1) (-1))::int64)" (is "?lhs = ?rhs")
+proof -
+  have "?rhs = -1 * (2 ^ (b-1))"
+    using push_bit_eq_mult by blast
+  also have "... = -(2 ^ (b-1))"
+    using mult_minus1 by blast
+  ultimately show ?thesis by simp
+qed
+
+lemma min_int_signed_neg2pow:
+  assumes "0 < b \<and> b \<le> 64"
+  shows "int_signed_value b (min_int b) = int_signed_value b (-(2^(b-1)))"
+  using assms
+  by (metis (no_types, lifting) One_nat_def diff_diff_cancel int_signed_value.simps le_simps(3) mask_1 mask_eq_take_bit_minus_one min_int_def min_int_push_bit or.left_neutral set_bit_def signed_take_take_bit take_bit_push_bit)
+
+definition max_int :: "nat \<Rightarrow> int64" where
+  "max_int bits = mask (bits - 1)"
+
+lemma max_int_mask:
+  assumes "0 < b \<and> b \<le> 64"
+  shows "(2 ^ (b - 1)) - 1 = ((mask (b-1))::int64)" (is "?lhs = ?rhs")
+  using assms
+  by (simp add: mask_eq_decr_exp)
+
+lemma max_int_signed_2pow:
+  assumes "0 < b \<and> b \<le> 64"
+  shows "int_signed_value b (max_int b) = int_signed_value b ((2 ^ (b - 1)) - 1)"
+  using assms
+  by (simp add: mask_eq_exp_minus_1 max_int_def)
+
+
+abbreviation javaLT :: "nat \<Rightarrow> int64 \<Rightarrow> int64 \<Rightarrow> bool" ("_ \<turnstile> _ <j _" 50) where
+  "javaLT b x y \<equiv> (int_signed_value b x < int_signed_value b y)"
+
+abbreviation javaLTE :: "nat \<Rightarrow> int64 \<Rightarrow> int64 \<Rightarrow> bool" ("_ \<turnstile> _ \<le>j _" 50) where
+  "javaLTE b x y \<equiv> (int_signed_value b x \<le> int_signed_value b y)"
+
 fun valid_stamp :: "Stamp \<Rightarrow> bool" where
-  "valid_stamp (IntegerStamp bits lo hi) = 
+  "valid_stamp (IntegerStamp bits lo hi down up) = 
      (0 < bits \<and> bits \<le> 64 \<and>
-     fst (bit_bounds bits) \<le> lo \<and> lo \<le> snd (bit_bounds bits) \<and>
-     fst (bit_bounds bits) \<le> hi \<and> hi \<le> snd (bit_bounds bits))" |
+     take_bit bits lo = lo \<and> (bits \<turnstile> (min_int bits) \<le>j lo) \<and> (bits \<turnstile> lo \<le>j (max_int bits)) \<and>
+     take_bit bits hi = hi \<and> (bits \<turnstile> (min_int bits) \<le>j hi) \<and> (bits \<turnstile> hi \<le>j (max_int bits)))" |
   "valid_stamp s = True"
 
 (* Note: we could support 32/64-bit unsigned values by relaxing this definition to:
@@ -66,7 +108,7 @@ fun valid_stamp :: "Stamp \<Rightarrow> bool" where
 *)
 
 experiment begin
-corollary "bit_bounds 1 = (-1, 0)" by simp  (* this matches the compiler stamps. *)
+corollary "int_signed_value 1 (min_int 1) = -1 \<and> max_int 1 = 0" by eval  (* this matches the compiler stamps. *)
 end
 
 (* NOTE: the FloatStamp has been commented out to allow use of code generation facilities *)
@@ -81,7 +123,7 @@ definition neg_infinity :: "float" where
 \<comment> \<open>A stamp which includes the full range of the type\<close>
 fun unrestricted_stamp :: "Stamp \<Rightarrow> Stamp" where
   "unrestricted_stamp VoidStamp = VoidStamp" |
-  "unrestricted_stamp (IntegerStamp bits lower upper) = (IntegerStamp bits (fst (bit_bounds bits)) (snd (bit_bounds bits)))" | 
+  "unrestricted_stamp (IntegerStamp bits lower upper down up) = (IntegerStamp bits (min_int bits) (max_int bits) 0 (mask bits))" | 
   (* "unrestricted_stamp (FloatStamp bits lower upper) = (FloatStamp bits neg_infinity pos_infinity)" |  *)
   "unrestricted_stamp (KlassPointerStamp nonNull alwaysNull) = (KlassPointerStamp False False)" |
   "unrestricted_stamp (MethodCountersPointerStamp nonNull alwaysNull) = (MethodCountersPointerStamp False False)" |
@@ -95,7 +137,7 @@ fun is_stamp_unrestricted :: "Stamp \<Rightarrow> bool" where
 \<comment> \<open>A stamp which provides type information but has an empty range of values\<close>
 fun empty_stamp :: "Stamp \<Rightarrow> Stamp" where
   "empty_stamp VoidStamp = VoidStamp" |
-  "empty_stamp (IntegerStamp bits lower upper) = (IntegerStamp bits (snd (bit_bounds bits)) (fst (bit_bounds bits)))" |
+  "empty_stamp (IntegerStamp bits lower upper down up) = (IntegerStamp bits (max_int bits) (min_int bits) (mask bits) 0)" |
   (* "empty_stamp (FloatStamp bits lower upper) = (FloatStamp bits pos_infinity neg_infinity)" | *)
   "empty_stamp (KlassPointerStamp nonNull alwaysNull) = (KlassPointerStamp nonNull alwaysNull)" |
   "empty_stamp (MethodCountersPointerStamp nonNull alwaysNull) = (MethodCountersPointerStamp nonNull alwaysNull)" |
@@ -103,13 +145,41 @@ fun empty_stamp :: "Stamp \<Rightarrow> Stamp" where
   "empty_stamp (ObjectStamp type exactType nonNull alwaysNull) = (ObjectStamp '''' True True False)" |
   "empty_stamp stamp = IllegalStamp"
 
+definition smin :: "nat \<Rightarrow> int64 \<Rightarrow> int64 \<Rightarrow> int64" where
+  "smin b x y = (if b \<turnstile> x \<le>j y then x else y)"
+
+definition smax :: "nat \<Rightarrow> int64 \<Rightarrow> int64 \<Rightarrow> int64" where
+  "smax b x y = (if b \<turnstile> x \<le>j y then y else x)"
+
+
+lemma signed_value_eq:
+  assumes "take_bit b x = x"
+  assumes "take_bit b y = y"
+  shows "int_signed_value b x = int_signed_value b y \<Longrightarrow> x = y"
+  unfolding int_signed_value.simps
+  by (smt (verit, best) Suc_pred' assms(1) assms(2) cancel_comm_monoid_add_class.diff_cancel less_imp_diff_less not_less signed_take_bit_eq_iff_take_bit_eq signed_take_bit_take_bit signed_word_eqI)
+
+lemma smin_commute:
+  assumes "take_bit b x = x"
+  assumes "take_bit b y = y"
+  shows "smin b x y = smin b y x"
+  unfolding smin_def
+  by (meson assms(1) assms(2) nle_le signed_value_eq)
+
+lemma smax_commute:
+  assumes "take_bit b x = x"
+  assumes "take_bit b y = y"
+  shows "smax b x y = smax b y x"
+  unfolding smax_def
+  by (meson assms(1) assms(2) nle_le signed_value_eq)
+
 
 \<comment> \<open>Calculate the meet stamp of two stamps\<close>
 fun meet :: "Stamp \<Rightarrow> Stamp \<Rightarrow> Stamp" where
   "meet VoidStamp VoidStamp = VoidStamp" |
-  "meet (IntegerStamp b1 l1 u1) (IntegerStamp b2 l2 u2) = (
+  "meet (IntegerStamp b1 l1 u1 d1 up1) (IntegerStamp b2 l2 u2 d2 up2) = (
     if b1 \<noteq> b2 then IllegalStamp else 
-    (IntegerStamp b1 (min l1 l2) (max u1 u2))
+    (IntegerStamp b1 (smin b1 l1 l2) (smax b1 u1 u2) (and d1 d2) (or up1 up2))
   )" |
   (* "meet (FloatStamp b1 l1 u1) (FloatStamp b2 l2 u2) = (
     if b1 \<noteq> b2 then IllegalStamp else 
@@ -129,9 +199,9 @@ fun meet :: "Stamp \<Rightarrow> Stamp \<Rightarrow> Stamp" where
 \<comment> \<open>Calculate the join stamp of two stamps\<close>
 fun join :: "Stamp \<Rightarrow> Stamp \<Rightarrow> Stamp" where
   "join VoidStamp VoidStamp = VoidStamp" |
-  "join (IntegerStamp b1 l1 u1) (IntegerStamp b2 l2 u2) = (
+  "join (IntegerStamp b1 l1 u1 d1 up1) (IntegerStamp b2 l2 u2 d2 up2) = (
     if b1 \<noteq> b2 then IllegalStamp else 
-    (IntegerStamp b1 (max l1 l2) (min u1 u2))
+    (IntegerStamp b1 (max l1 l2) (min u1 u2) (or d1 d2) (and up1 up2))
   )" |
   (* "join (FloatStamp b1 l1 u1) (FloatStamp b2 l2 u2) = (
     if b1 \<noteq> b2 then IllegalStamp else 
@@ -160,7 +230,7 @@ the asConstant function converts the stamp to a value where one can be inferred.
 \<close>
 (* NOTE: we could also add a 32-bit version of this if needed. *)
 fun asConstant :: "Stamp \<Rightarrow> Value" where
-  "asConstant (IntegerStamp b l h) = (if l = h then new_int b (word_of_int l) else UndefVal)" |
+  "asConstant (IntegerStamp b l h d u) = (if l = h then new_int b l else UndefVal)" |
   "asConstant _ = UndefVal"
 
 \<comment> \<open>Determine if two stamps never have value overlaps i.e. their join is empty\<close>
@@ -172,7 +242,7 @@ fun neverDistinct :: "Stamp \<Rightarrow> Stamp \<Rightarrow> bool" where
   "neverDistinct stamp1 stamp2 = (asConstant stamp1 = asConstant stamp2 \<and> asConstant stamp1 \<noteq> UndefVal)"
 
 fun constantAsStamp :: "Value \<Rightarrow> Stamp" where
-  "constantAsStamp (IntVal b v) = (IntegerStamp b (int_signed_value b v) (int_signed_value b v))" |
+  "constantAsStamp (IntVal b v) = (IntegerStamp b (take_bit b v) (take_bit b v) (and v (mask b)) (and v (mask b)))" |
   "constantAsStamp (ObjRef (None)) = ObjectStamp '''' False False True" |
   "constantAsStamp (ObjRef (Some n)) = ObjectStamp '''' False True False" |
   (* TODO: float *)
@@ -181,11 +251,13 @@ fun constantAsStamp :: "Value \<Rightarrow> Stamp" where
 \<comment> \<open>Define when a runtime value is valid for a stamp.
     The stamp bounds must be valid, and val must be zero-extended.\<close>
 fun valid_value :: "Value \<Rightarrow> Stamp \<Rightarrow> bool" where
-  "valid_value (IntVal b1 val) (IntegerStamp b l h) =
+  "valid_value (IntVal b1 val) (IntegerStamp b l h d u) =
      (if b1 = b then
-       valid_stamp (IntegerStamp b l h) \<and>
+       valid_stamp (IntegerStamp b l h d u) \<and>
        take_bit b val = val \<and>
-       l \<le> int_signed_value b val \<and> int_signed_value b val \<le> h
+       (b \<turnstile> l \<le>j val) \<and> (b \<turnstile> val \<le>j h) \<and>
+       (and (not val) d) = 0 \<and>
+       (and val u) = val
       else False)" |
   (* "valid_value (FloatStamp b1 l h) (FloatVal b2 v) = ((b1 = b2) \<and> (v \<ge> l) \<and> (v \<le> h))" | *)
   "valid_value (ObjRef ref) (ObjectStamp klass exact nonNull alwaysNull) = 
@@ -221,14 +293,16 @@ lemma unfold_wf_value[simp]:
   "wf_value v \<Longrightarrow> valid_value v (constantAsStamp v)"
   by (simp add: wf_value_def)
 
+declare [[linarith_split_limit=20]] (* TODO: worrying *)
 fun compatible :: "Stamp \<Rightarrow> Stamp \<Rightarrow> bool" where
-  "compatible (IntegerStamp b1 lo1 hi1) (IntegerStamp b2 lo2 hi2) =
-     (b1 = b2 \<and> valid_stamp (IntegerStamp b1 lo1 hi1) \<and> valid_stamp (IntegerStamp b2 lo2 hi2))" |
+  "compatible (IntegerStamp b1 lo1 hi1 d1 u1) (IntegerStamp b2 lo2 hi2 d2 u2) =
+     (b1 = b2 \<and> valid_stamp (IntegerStamp b1 lo1 hi1 d1 u1) \<and> valid_stamp (IntegerStamp b2 lo2 hi2 d2 u2))" |
   "compatible (VoidStamp) (VoidStamp) = True" |
   "compatible _ _ = False"
+declare [[linarith_split_limit=9]]
 
 fun stamp_under :: "Stamp \<Rightarrow> Stamp \<Rightarrow> bool" where
-  "stamp_under (IntegerStamp b1 lo1 hi1) (IntegerStamp b2 lo2 hi2) = (hi1 < lo2)" |
+  "stamp_under (IntegerStamp b1 lo1 hi1 d1 u1) (IntegerStamp b2 lo2 hi2 d2 u2) = ((b1 = b2) \<and> (b1 \<turnstile> hi1 <j lo2))" |
   "stamp_under _ _ = False"
 
 \<comment> \<open>
@@ -236,7 +310,16 @@ The most common type of stamp within the compiler (apart from the VoidStamp) is 
 integer stamp with an unrestricted range. We use @{text default_stamp} as it is a frequently used stamp.
 \<close>
 definition default_stamp :: "Stamp" where
-  "default_stamp = (unrestricted_stamp (IntegerStamp 32 0 0))"
+  "default_stamp = (unrestricted_stamp (IntegerStamp 32 0 0 0 0))"
 
-value "valid_value (IntVal 8 (255)) (IntegerStamp 8 (-128) 127)"
+value "valid_value (IntVal 8 (255)) (IntegerStamp 8 (-128) 127 (mask 8) 0)"
+value "default_stamp"
+value "sint (min_int 32)"
+value "255 \<le>s max_int 32"
+value "min_int 32 \<le>s 255"
+value "mask 32::int64"
+value "and (not 255) (0::64 word) = 0"
+value "((and 255 (not (mask 32)))::int64) = 0"
+value "valid_stamp default_stamp"
+value "valid_value (IntVal 32 (255)) default_stamp"
 end
